Proved existence of a normal form

NormalForm.v
@@ -79,3 +79,115 @@ Proof.
     apply reduction_strongly_confluent.
 Qed.
 
+Fixpoint inv { T : Type } (x : WithInv T) : WithInv T
+    := match x with
+     | Reg    _ a => ForInv T a
+     | ForInv _ a => Reg    T a
+    end.
+
+Inductive is_stable { T : Type } : FreeMonT (WithInv T) -> Prop
+    := StableEmpty : is_stable (Empty (WithInv T))
+    |  StableSing : forall (x : WithInv T), is_stable (App (WithInv T) x (Empty (WithInv T)))
+    |  StableApp : forall (x y : WithInv T), forall (w : FreeMonT (WithInv T)),
+            inv x <> y -> is_stable (App (WithInv T) y w)
+                -> is_stable (App (WithInv T) x (App (WithInv T) y w)).
+
+Lemma normal_form_sub { T : Type } :
+    forall (x : WithInv T), forall (w : FreeMonT (WithInv T)),
+        normal_form (Reduction T) (App (WithInv T) x w) -> normal_form (Reduction T) w.
+Proof.
+    intros x w Hnf. unfold normal_form. intros w' Hred.
+    apply (Hnf (App (WithInv T) x w')). apply CtxRed.
+    assumption.
+Qed.
+
+Theorem stable_is_normal_form { T : Type } :
+    forall (x : FreeMonT (WithInv T)), is_stable x <-> normal_form (Reduction T) x.
+Proof.
+    intro x. split.
+    - intro Hstable. induction Hstable.
+      + unfold normal_form. intros x Hred. inversion Hred.
+      + unfold normal_form. intros w Hred. inversion Hred. inversion H2.
+      + unfold normal_form. intros w' Hred.
+        remember (App (WithInv T) y w) as tl0.
+        remember (App (WithInv T) x tl0) as tl1.
+        destruct Hred.
+        * rewrite -> Heqtl0 in Heqtl1. inversion Heqtl1.
+          apply H. rewrite <- H1. rewrite <- H2. reflexivity.
+        * rewrite -> Heqtl0 in Heqtl1. inversion Heqtl1.
+          apply H. rewrite <- H1. rewrite <- H2. reflexivity.
+        * unfold normal_form in IHHstable. apply (IHHstable m').
+          inversion Heqtl1. rewrite <- H2. assumption.
+
+    - intro Hnf. induction x; try constructor. destruct x.
+      + apply StableApp.
+        * intro Heq. destruct t.
+          { apply (Hnf x). rewrite <- Heq. apply RightRed. }
+          { apply (Hnf x). rewrite <- Heq. apply LeftRed. }
+        * apply IHx. apply (normal_form_sub t). assumption.
+      + apply StableSing.
+Qed.
+
+Axiom axiom_K_is_stable :
+    forall (T : Type), forall (w : FreeMonT (WithInv T)), forall (p1 p2 : is_stable w), p1 = p2.
+
+Definition DecEq (T : Type) : Type := forall (a b : T), { a = b } + { a <> b }.
+
+Lemma deceq_within { T : Type } (deceq : DecEq T) : DecEq (WithInv T).
+Proof.
+    unfold DecEq. intros a b. destruct a; destruct b.
+    - destruct (deceq t t0).
+      * left. rewrite e. reflexivity.
+      * right. intro H. apply n. inversion H. reflexivity.
+    - right. intro H. inversion H.
+    - right. intro H. inversion H.
+    - destruct (deceq t t0).
+      * left. rewrite e. reflexivity.
+      * right. intro H. apply n. inversion H. reflexivity.
+Qed.
+
+Theorem has_red_or_is_nf { T : Type } (deceq : DecEq T) :
+    forall (w : FreeMonT (WithInv T)), normal_form (Reduction T) w
+        \/ exists (w' : FreeMonT (WithInv T)), Reduction T w w'.
+Proof.
+    intro w. induction w.
+    - destruct w.
+      + destruct (deceq_within deceq (inv t) w).
+        * destruct t.
+          { right. rewrite <- e. exists w0. apply RightRed. }
+          { right. rewrite <- e. exists w0. apply LeftRed. }
+        * destruct IHw.
+          { left. intros w1 Hred. remember (App (WithInv T) t (App (WithInv T) w w0)) as w'. destruct Hred.
+            - apply n. inversion Heqw'. reflexivity.
+            - apply n. inversion Heqw'. reflexivity.
+            - inversion Heqw'. apply (H m'). rewrite <- H2. assumption.
+          }
+          { right. destruct H as [ w' Hred ]. exists (App (WithInv T) t w'). apply CtxRed. assumption. }
+      + left. intros w' Hred. inversion Hred. inversion H2.
+    - left. intros w Hred. inversion Hred.
+Qed.
+
+Theorem nf_exists' { T : Type } (deceq : DecEq T) :
+    forall (a : FreeMonT (WithInv T)),
+        (forall (b : FreeMonT (WithInv T)), Reduction T a b ->
+            exists (nf : FreeMonT (WithInv T)), trefl_closure (Reduction T) b nf /\ normal_form (Reduction T) nf)
+    -> exists (nf : FreeMonT (WithInv T)), trefl_closure (Reduction T) a nf /\ normal_form (Reduction T) nf.
+Proof.
+    intros a H. destruct (has_red_or_is_nf deceq a).
+    - exists a. split; try constructor. assumption.
+    - destruct H0 as [ b Hred ]. destruct (H b Hred) as [ nf [ Hrefl Hnf ] ].
+      exists nf. split; try assumption. apply (TransClosure (Reduction T) a b); assumption.
+Qed.
+
+Theorem nf_exists { T : Type } (deceq : DecEq T) :
+    forall (a : FreeMonT (WithInv T)),
+        exists (nf : FreeMonT (WithInv T)), trefl_closure (Reduction T) a nf /\ normal_form (Reduction T) nf.
+Proof.
+    apply (well_founded_ind (reduction_normalizing T)).
+    apply nf_exists'. assumption.
+Qed.
+
+
+
+
+
